BranchingAssembly/Debranching.thy
@@ -36,62 +36,56 @@ definition debranch :: "b_assembly_program \<Rightarrow> assembly_program" where
 
 function remove_continuations :: "assembly list \<Rightarrow> code_label \<Rightarrow> assembly_program \<Rightarrow> 
     (assembly list \<times> code_label) set" where
-  "remove_continuations \<pi> s \<Pi> = (
-    if finite (dom \<Pi>)
-    then case \<Pi> s of 
+  "\<not> finite (dom \<Pi>) \<Longrightarrow> remove_continuations \<pi> s \<Pi> = {(\<pi>, s)}"
+| "finite (dom \<Pi>) \<Longrightarrow> remove_continuations \<pi> s \<Pi> = (case \<Pi> s of 
         Some (\<pi>', s') \<Rightarrow> insert (\<pi>, s) (remove_continuations (\<pi> @ \<pi>') s' (\<Pi>(s := None)))
-      | None \<Rightarrow> {(\<pi>, s)}
-    else {(\<pi>, s)})"
-  by pat_completeness auto
+      | None \<Rightarrow> {(\<pi>, s)})"
+  by atomize_elim auto
 termination
   by (relation "measure (card o dom o snd o snd)") (auto, meson card_Diff1_less domI)
 
 fun state_convert :: "code_label set \<Rightarrow> b_assembly_state \<Rightarrow> assembly_state set" where
   "state_convert ss (\<mu>, a, d, \<pi>, s, \<omega>) = (
-    let (\<pi>', s', \<Pi>) = branch_instr_convert ss \<pi> s
-    in {(\<mu>, a, d, \<pi>'', s'', \<omega>) | \<pi>'' s''. (\<pi>'', s'') \<in> remove_continuations \<pi>' s' \<Pi>})"
+    let (\<pi>', s', \<Pi>') = branch_instr_convert ss \<pi> s
+    in {(\<mu>, a, d, \<pi>'', s'', \<omega>) | \<pi>'' s''. (\<pi>'', s'') \<in> remove_continuations \<pi>' s' \<Pi>'})"
 
 (* conversion correctness *)
 
-lemma [simp]: "branch_instr_convert ss \<pi>\<^sub>B = (\<pi>\<^sub>A, \<Pi>) \<Longrightarrow> finite ss \<Longrightarrow> finite (dom \<Pi>)"
-  proof (induction ss \<pi>\<^sub>B arbitrary: \<pi>\<^sub>A \<Pi> rule: branch_instr_convert.induct)
+lemma [simp]: "branch_instr_convert ss \<pi>\<^sub>B s = (\<pi>\<^sub>A, s', \<Pi>) \<Longrightarrow> finite ss \<Longrightarrow> finite (dom \<Pi>)"
+  proof (induction ss \<pi>\<^sub>B s arbitrary: \<pi>\<^sub>A s' \<Pi> rule: branch_instr_convert.induct)
   case 1
     thus ?case by auto
   next case 2
     thus ?case by (simp split: prod.splits)
   next case 3
     thus ?case by (simp split: prod.splits)
-  next case (4 ss jmp \<pi>\<^sub>B\<^sub>t \<pi>\<^sub>B\<^sub>f \<pi>\<^sub>B)
-    thus ?case
-      proof (cases "branch_instr_convert ss \<pi>\<^sub>B\<^sub>t")
-      case (Pair \<pi>\<^sub>A\<^sub>t \<Pi>\<^sub>1) note PT = Pair
-        thus ?thesis  
-          proof (cases "branch_instr_convert (ss \<union> dom \<Pi>\<^sub>1) \<pi>\<^sub>B\<^sub>f")
-          case (Pair \<pi>\<^sub>A\<^sub>f \<Pi>\<^sub>2) note PF = Pair
+  next case (4 ss jmp \<pi>\<^sub>B\<^sub>t \<pi>\<^sub>B\<^sub>f \<pi>\<^sub>B s)
+    let ?s\<^sub>e = "new_label ss"
+    have "finite (dom \<Pi>)"
+      proof (cases "branch_instr_convert (ss \<union> {?s\<^sub>e}) \<pi>\<^sub>B\<^sub>t ?s\<^sub>e")
+      case (fields \<pi>\<^sub>t' s\<^sub>t \<Pi>\<^sub>1) note F1 = fields
+        thus ?thesis
+          proof (cases "branch_instr_convert (ss \<union> dom \<Pi>\<^sub>1 \<union> {?s\<^sub>e}) \<pi>\<^sub>B\<^sub>f ?s\<^sub>e")
+          case (fields \<pi>\<^sub>f' s\<^sub>f \<Pi>\<^sub>2) note F2 = fields
             thus ?thesis
-              proof (cases "branch_instr_convert (ss \<union> dom \<Pi>\<^sub>1 \<union> dom \<Pi>\<^sub>2) \<pi>\<^sub>B")
-              case (Pair \<pi>\<^sub>A' \<Pi>\<^sub>3)
-                let ?s\<^sub>t = "new_label (ss \<union> dom \<Pi>\<^sub>1 \<union> dom \<Pi>\<^sub>2 \<union> dom \<Pi>\<^sub>3)"
-                let ?s\<^sub>e = "new_label (ss \<union> dom \<Pi>\<^sub>1 \<union> dom \<Pi>\<^sub>2 \<union> dom \<Pi>\<^sub>3 \<union> {?s\<^sub>t})"
-                from 4 PT PF Pair have "finite (dom (\<Pi>\<^sub>1 ++ \<Pi>\<^sub>2 ++ \<Pi>\<^sub>3 ++ 
-                  [?s\<^sub>t \<mapsto> \<pi>\<^sub>A\<^sub>t @ [JAssm {EQ, LT, GT} ?s\<^sub>e], ?s\<^sub>e \<mapsto> \<pi>\<^sub>A']))" by simp
-                with 4 PT PF Pair show ?thesis by (simp add: Let_def)
+              proof (cases "branch_instr_convert (ss \<union> dom \<Pi>\<^sub>1 \<union> dom \<Pi>\<^sub>2 \<union> {?s\<^sub>e}) \<pi>\<^sub>B s")
+              case (fields \<pi>' s'' \<Pi>\<^sub>3)
+                with 4 F1 F2 fields show ?thesis by auto
               qed
           qed
       qed
+    thus ?case by simp
   next case 5
-    thus ?case by auto
-  next case 6
     thus ?case by (simp split: prod.splits)
   qed
 
 lemma finite_block_convert: "finite (dom \<Pi>) \<Longrightarrow> finite ss \<Longrightarrow> 
-    finite (dom (block_convert ss (s, \<pi>) \<Pi>))"
-  by (cases "branch_instr_convert (ss \<union> dom \<Pi>) \<pi>") auto
+    finite (dom (block_convert ss \<pi> \<Pi>))"
+  by (cases \<pi>) (auto split: prod.splits)
 
 lemma [simp]: "finite ss \<Longrightarrow> ss \<supseteq> dom \<Pi> \<Longrightarrow> 
     finite (dom (finite_map_fold (block_convert ss) empty \<Pi>))"
-  proof (induction "block_convert ss" "empty :: code_label \<Rightarrow> assembly list option" \<Pi> 
+  proof (induction "block_convert ss" "empty :: code_label \<Rightarrow> (assembly list \<times> code_label) option" \<Pi> 
          rule: finite_map_fold.induct)
   case 1
     thus ?case by (metis finite_subset)
@@ -108,44 +102,21 @@ lemma [simp]: "finite ss \<Longrightarrow> ss \<supseteq> dom \<Pi> \<Longrighta
 lemma [simp]: "finite (dom \<Pi>) \<Longrightarrow> finite (dom (debranch \<Pi>))"
   by (simp add: debranch_def)
 
-lemma [simp]: "\<pi> \<in> jump_join \<pi> \<Pi>"
-  by (cases "last \<pi>") (simp_all split: option.splits)
+lemma [simp]: "(\<pi>, s) \<in> remove_continuations \<pi> s \<Pi>"
+  by (induction \<pi> s \<Pi> rule: remove_continuations.induct) (simp_all split: option.splits)
 
-lemma jump_join_a: "\<pi>' \<in> jump_join (AAssm x # \<pi>) \<Pi> \<Longrightarrow> 
-    \<exists>\<pi>''. \<pi>' = AAssm x # \<pi>'' \<and> \<pi>'' \<in> jump_join \<pi> \<Pi>"
-  proof (induction "AAssm x # \<pi>" \<Pi> rule: jump_join.induct)
-  case (1 \<Pi>)
+lemma remove_cont_extends: "(\<pi>', s') \<in> remove_continuations (\<iota> # \<pi>) s \<Pi> \<Longrightarrow> 
+    \<exists>\<pi>''. \<pi>' = \<iota> # \<pi> @ \<pi>'' \<and> (\<pi> @ \<pi>'', s') \<in> remove_continuations \<pi> s \<Pi>"
+  proof (induction \<pi> s \<Pi> rule: remove_continuations.induct)
+  case 1
+    thus ?case by simp
+  next case (2 \<Pi> \<pi> s)
     thus ?case
-      proof (cases "finite (dom \<Pi>)")
-      case True
-        from 1 True have "
-            last (AAssm x # \<pi>) = JAssm jmp s \<Longrightarrow>
-            jmp = {GT, EQ, LT} \<Longrightarrow>
-            \<Pi> s = Some pi \<Longrightarrow>
-            butlast (AAssm x # \<pi>) @ pi = AAssm x # \<pi> \<Longrightarrow> \<pi>' \<in> jump_join (AAssm x # \<pi>) (\<Pi>(s := None)) \<Longrightarrow> \<exists>\<pi>''. \<pi>' = AAssm x # \<pi>'' \<and> \<pi>'' \<in> jump_join \<pi> (\<Pi>(s := None))" by simp
-        from 1 True have "\<pi>' \<in> (
-        case last (AAssm x # \<pi>) of
-            JAssm jmp s \<Rightarrow> (
-              if jmp = {GT, EQ, LT} 
-              then case \<Pi> s of 
-                  Some \<pi>' \<Rightarrow> insert (AAssm x # \<pi>) (jump_join (butlast (AAssm x # \<pi>) @ \<pi>') (\<Pi>(s := None)))
-                | None \<Rightarrow> {AAssm x # \<pi>} 
-              else {AAssm x # \<pi>})
-          | _ \<Rightarrow> {AAssm x # \<pi>})" by simp
-    
-    
-        have "\<pi>' = AAssm x # \<pi>'' \<and> \<pi>'' \<in> (
-        case last \<pi> of
-            JAssm jmp s \<Rightarrow> (
-              if jmp = {GT, EQ, LT} 
-              then case \<Pi> s of 
-                  Some \<pi>' \<Rightarrow> insert \<pi> (jump_join (butlast \<pi> @ \<pi>') (\<Pi>(s := None)))
-                | None \<Rightarrow> {\<pi>} 
-              else {\<pi>})
-          | _ \<Rightarrow> {\<pi>})" by simp
-        with True show ?thesis by simp
-      next case False
-        with 1 show ?thesis by simp
+      proof (cases "\<Pi> s")
+      case (Some ps)
+        with 2 show ?thesis by (cases ps) fastforce
+      next case None
+        with 2 show ?thesis by simp
       qed
   qed
 
@@ -153,27 +124,101 @@ lemma [simp]: "\<Sigma>\<^sub>A \<in> state_convert ss \<Sigma>\<^sub>B \<Longri
   by (induction \<Sigma>\<^sub>B rule: b_assembly_output.induct, induction \<Sigma>\<^sub>A rule: assembly_output.induct) 
      (simp split: prod.splits)
 
-lemma debranch_step: "eval_b_assembly \<Pi> \<Sigma>\<^sub>B = Some \<Sigma>\<^sub>B' \<Longrightarrow> finite (dom \<Pi>) \<Longrightarrow> 
-  \<Sigma>\<^sub>A \<in> state_convert (dom \<Pi>) \<Sigma>\<^sub>B \<Longrightarrow> 
-    \<exists>\<Sigma>\<^sub>A'. \<Sigma>\<^sub>A' \<in> state_convert (dom \<Pi>) \<Sigma>\<^sub>B' \<and> iterate (eval_assembly (debranch \<Pi>)) \<Sigma>\<^sub>A \<Sigma>\<^sub>A'"
+lemma debranch_step: "eval_b_assembly \<Pi> \<Sigma>\<^sub>B = Some \<Sigma>\<^sub>B' \<Longrightarrow> \<Sigma>\<^sub>A \<in> state_convert (dom \<Pi>) \<Sigma>\<^sub>B \<Longrightarrow> 
+    \<exists>\<Sigma>\<^sub>A'. \<Sigma>\<^sub>A' \<in> state_convert (dom \<Pi>) \<Sigma>\<^sub>B' \<and> eval_assembly (debranch \<Pi>) \<Sigma>\<^sub>A = Some \<Sigma>\<^sub>A'"
   proof (induction \<Pi> \<Sigma>\<^sub>B rule: eval_b_assembly.induct)
-  case 1
-    thus ?case by simp
-  next case (2 \<Pi> \<mu> a d x \<pi> \<omega>)
-    thus ?case by simp
-  next case (3 \<Pi> \<mu> a d dst cmp \<pi> \<omega>)
-    thus ?case by simp
+  case (1 \<Pi> \<mu> a d s \<omega>)
+    thus ?case
+      proof (cases "\<Pi> s")
+      case (Some ps)
+        thus ?thesis
+          proof (cases ps)
+          case (Pair \<pi>\<^sub>B s')
+            thus ?thesis
+              proof (cases "branch_instr_convert (dom \<Pi>) \<pi>\<^sub>B s'")
+              case (fields \<pi>\<^sub>A s'' \<Pi>')
+
+            
+                have X: "\<Sigma>\<^sub>A' \<in> state_convert (dom \<Pi>) (\<mu>, None, d, \<pi>\<^sub>B, s', \<omega>)" by simp
+    
+    
+                have "(case debranch \<Pi> s of 
+      Some (\<pi>', s') \<Rightarrow> Some (\<mu>, None, d, \<pi>', s', \<omega>)
+    | None \<Rightarrow> None) = Some \<Sigma>\<^sub>A'" by simp
+                with X 1 Some Pair fields show ?thesis by auto
+              qed
+          qed
+      next case None
+        with 1 show ?thesis by simp
+      qed
+  next case (2 \<Pi> \<mu> a d x \<pi>\<^sub>B s \<omega>)
+    with remove_cont_extends show ?case by (cases "branch_instr_convert (dom \<Pi>) \<pi>\<^sub>B s") fastforce
+  next case (3 \<Pi> \<mu> a d dst cmp \<pi>\<^sub>B s \<omega>)
+    thus ?case
+      proof (cases "branch_instr_convert (dom \<Pi>) \<pi>\<^sub>B s")
+      case (fields \<pi>\<^sub>A s' \<Pi>')
+        let ?n = "compute cmp (\<mu> a) a d"
+        let ?m = "if M \<in> dst then \<mu>(a := ?n) else \<mu>"
+        let ?a = "Some (if A \<in> dst then ?n else a)"
+        let ?d = "if D \<in> dst then ?n else d"
+        from 3 have SB: "\<Sigma>\<^sub>B' = (?m, ?a, ?d, \<pi>\<^sub>B, s, \<omega>)" by (simp add: Let_def)
+        from 3 fields obtain \<pi>\<^sub>A' s'' where SA: "\<Sigma>\<^sub>A = (\<mu>, Some a, d, \<pi>\<^sub>A', s'', \<omega>) \<and> 
+          (\<pi>\<^sub>A', s'') \<in> remove_continuations (CAssm dst cmp # \<pi>\<^sub>A) s' \<Pi>'" by fastforce
+        with remove_cont_extends obtain \<pi>\<^sub>A'' where P: "\<pi>\<^sub>A' = CAssm dst cmp # \<pi>\<^sub>A @ \<pi>\<^sub>A'' \<and> 
+          (\<pi>\<^sub>A @ \<pi>\<^sub>A'', s'') \<in> remove_continuations \<pi>\<^sub>A s' \<Pi>'" by fastforce
+        have "eval_assembly (debranch \<Pi>) (\<mu>, Some a, d, CAssm dst cmp # \<pi>\<^sub>A @ \<pi>\<^sub>A'', s'', \<omega>) = 
+          Some (?m, ?a, ?d, \<pi>\<^sub>A @ \<pi>\<^sub>A'', s'', \<omega>)" by (simp add: Let_def)
+        with 3 SA SB P fields show ?thesis by fastforce
+      qed
   next case 4
     thus ?case by simp
-  next case (5 \<Pi> \<mu> a d jmp \<pi>\<^sub>t \<pi>\<^sub>f \<pi> \<omega>)
-    thus ?case by simp
-  next case (6 \<Pi> \<mu> a d s \<pi> \<omega>)
-    thus ?case by simp
-  next case (7 \<Pi> \<mu> a d \<pi> \<omega>)
-    thus ?case by simp
+  next case (5 \<Pi> \<mu> a d jmp \<pi>\<^sub>B\<^sub>t \<pi>\<^sub>B\<^sub>f \<pi>\<^sub>B s \<omega>)
+    let ?s\<^sub>e = "new_label (dom \<Pi>)"
+    show ?case
+      proof (cases "branch_instr_convert (dom \<Pi> \<union> {?s\<^sub>e}) \<pi>\<^sub>B\<^sub>t ?s\<^sub>e")
+      case (fields \<pi>\<^sub>t' s\<^sub>t \<Pi>\<^sub>1) note BE = fields
+        thus ?thesis
+          proof (cases "branch_instr_convert (dom \<Pi> \<union> dom \<Pi>\<^sub>1 \<union> {?s\<^sub>e}) \<pi>\<^sub>B\<^sub>f ?s\<^sub>e")
+          case (fields \<pi>\<^sub>f' s\<^sub>f \<Pi>\<^sub>2) note BF = fields
+            thus ?thesis
+              proof (cases "branch_instr_convert (dom \<Pi> \<union> dom \<Pi>\<^sub>1 \<union> dom \<Pi>\<^sub>2 \<union> {?s\<^sub>e}) \<pi>\<^sub>B s")
+              case (fields \<pi>' s' \<Pi>\<^sub>3)
+                thus ?thesis
+                  proof (cases "should_jump d jmp")
+                  case True
+                    from 5 True have SB: "\<Sigma>\<^sub>B' = (\<mu>, a, d, \<pi>\<^sub>B\<^sub>t @ \<pi>\<^sub>B, s, \<omega>)" by simp
+                    from 5 have SA: "\<Sigma>\<^sub>A \<in> state_convert (dom \<Pi>) (\<mu>, a, d, IBAssm jmp \<pi>\<^sub>B\<^sub>t \<pi>\<^sub>B\<^sub>f # \<pi>\<^sub>B, s, \<omega>)" by simp
+                
+            from BE BF fields have "state_convert (dom \<Pi>) (\<mu>, a, d, IBAssm jmp \<pi>\<^sub>B\<^sub>t \<pi>\<^sub>B\<^sub>f # \<pi>\<^sub>B, s, \<omega>) = (
+                let (\<pi>', s', \<Pi>') = (JAssm jmp s\<^sub>t # \<pi>\<^sub>f', s\<^sub>f, \<Pi>\<^sub>1 ++ \<Pi>\<^sub>2 ++ \<Pi>\<^sub>3 ++ [s\<^sub>t \<mapsto> (\<pi>\<^sub>t', s\<^sub>t), ?s\<^sub>e \<mapsto> (\<pi>', s')])
+                in {(\<mu>, a, d, \<pi>'', s'', \<omega>) | \<pi>'' s''. (\<pi>'', s'') \<in> remove_continuations (JAssm jmp s\<^sub>t # \<pi>\<^sub>f') s\<^sub>f \<Pi>'})" by (simp add: Let_def)
+            
+                
+            
+                    have X: "\<Sigma>\<^sub>A' \<in> state_convert (dom \<Pi>) (\<mu>, a, d, \<pi>\<^sub>B\<^sub>t @ \<pi>\<^sub>B, s, \<omega>)" by simp
+                
+                
+                    have "eval_assembly (debranch \<Pi>) \<Sigma>\<^sub>A = Some \<Sigma>\<^sub>A'" by simp
+                    with SB SA X show ?thesis by metis
+                  next case False
+                    from 5 False have SB: "\<Sigma>\<^sub>B' = (\<mu>, a, d, \<pi>\<^sub>B\<^sub>f @ \<pi>\<^sub>B, s, \<omega>)" by fastforce
+                    from 5 have "\<Sigma>\<^sub>A \<in> state_convert (dom \<Pi>) (\<mu>, a, d, IBAssm jmp \<pi>\<^sub>B\<^sub>t \<pi>\<^sub>B\<^sub>f # \<pi>\<^sub>B, s, \<omega>)" by simp
+                
+                
+                    have X: "\<Sigma>\<^sub>A' \<in> state_convert (dom \<Pi>) (\<mu>, a, d, \<pi>\<^sub>B\<^sub>f @ \<pi>\<^sub>B, s, \<omega>)" by simp
+                
+                
+                    have "eval_assembly (debranch \<Pi>) \<Sigma>\<^sub>A = Some \<Sigma>\<^sub>A'" by simp
+                    with SB X show ?thesis by metis
+                  qed
+              qed
+          qed
+      qed
+  next case (6 \<Pi> \<mu> a d \<pi>\<^sub>B s \<omega>)
+    with remove_cont_extends show ?case by (cases "branch_instr_convert (dom \<Pi>) \<pi>\<^sub>B s") fastforce
   qed 
 
-theorem debranching_correct [simp]: "iterate (eval_b_assembly \<Pi>) \<Sigma>\<^sub>B \<Sigma>\<^sub>B' \<Longrightarrow> finite (dom \<Pi>) \<Longrightarrow>
+theorem debranching_correct [simp]: "iterate (eval_b_assembly \<Pi>) \<Sigma>\<^sub>B \<Sigma>\<^sub>B' \<Longrightarrow> 
   \<Sigma>\<^sub>A \<in> state_convert (dom \<Pi>) \<Sigma>\<^sub>B \<Longrightarrow> 
     \<exists>\<Sigma>\<^sub>A'. \<Sigma>\<^sub>A' \<in> state_convert (dom \<Pi>) \<Sigma>\<^sub>B' \<and> iterate (eval_assembly (debranch \<Pi>)) \<Sigma>\<^sub>A \<Sigma>\<^sub>A'"
   proof (induction "eval_b_assembly \<Pi>" \<Sigma>\<^sub>B \<Sigma>\<^sub>B' rule: iterate.induct)
@@ -183,7 +228,7 @@ theorem debranching_correct [simp]: "iterate (eval_b_assembly \<Pi>) \<Sigma>\<^
     then obtain \<Sigma>\<^sub>A' where S: "\<Sigma>\<^sub>A' \<in> state_convert (dom \<Pi>) \<Sigma>\<^sub>B' \<and> 
       iterate (eval_assembly (debranch \<Pi>)) \<Sigma>\<^sub>A \<Sigma>\<^sub>A'" by blast
     with iter_step debranch_step obtain \<Sigma>\<^sub>A'' where
-      "\<Sigma>\<^sub>A'' \<in> state_convert (dom \<Pi>) \<Sigma>\<^sub>B'' \<and> iterate (eval_assembly (debranch \<Pi>)) \<Sigma>\<^sub>A' \<Sigma>\<^sub>A''" by blast
+      "\<Sigma>\<^sub>A'' \<in> state_convert (dom \<Pi>) \<Sigma>\<^sub>B'' \<and> eval_assembly (debranch \<Pi>) \<Sigma>\<^sub>A' = Some \<Sigma>\<^sub>A''" by blast
     with S have "\<Sigma>\<^sub>A'' \<in> state_convert (dom \<Pi>) \<Sigma>\<^sub>B'' \<and> iterate (eval_assembly (debranch \<Pi>)) \<Sigma>\<^sub>A \<Sigma>\<^sub>A''" 
       by fastforce
     thus ?case by blast
